progs/sha_lemmas.v
@@ -1,0 +1,279 @@
+Require Import proofauto.
+Require Import progs.SHA256.
+
+Definition big_endian_integer (contents: Z -> int) : int :=
+  Int.or (Int.shl (contents 3) (Int.repr 24))
+  (Int.or (Int.shl (contents 2) (Int.repr 16))
+   (Int.or (Int.shl (contents 1) (Int.repr 8))
+      (contents 0))).
+
+Open Scope nat.
+
+Definition LBLOCK : nat := 16.   (* length of a block, in 32-bit integers *)
+Definition CBLOCK : nat := LBLOCK * 4.  (* length of a block, in characters *)
+
+
+Definition s256state := (list int * (int * (int * (list int * int))))%type.
+Definition s256_h (s: s256state) := fst s.
+Definition s256_Nl (s: s256state) := fst (snd s).
+Definition s256_Nh (s: s256state) := fst (snd (snd s)).
+Definition s256_data (s: s256state) := fst (snd (snd (snd s))).
+Definition s256_num (s: s256state) := snd (snd (snd (snd s))).
+
+Inductive s256abs :=  (* SHA-256 abstract state *)
+ S256abs: forall (hashed: list int)   (* words hashed, so far *)
+                         (delta: nat) (* length of "hashed" minus the recorded length in hl *)
+                         (data: list Z)  (* bytes in the partial block not yet hashed *),
+                     s256abs.
+
+Definition s256_relate (a: s256abs) (r: s256state) : Prop :=
+     match a with S256abs hashed delta data =>
+         s256_h r = process_msg init_registers hashed 
+       /\ length (intlist_to_Zlist hashed) = 
+             delta + Z.to_nat (Int.unsigned (s256_Nh r) * Int.modulus + Int.unsigned (s256_Nl r))
+       /\ data = map Int.unsigned (firstn (Z.to_nat (Int.unsigned (s256_num r))) (s256_data r))
+       /\ length data < CBLOCK
+       /\ (exists n, length hashed = 16*n)
+       /\ length (s256_data r) = CBLOCK
+     end.
+
+
+Lemma length_map2:
+ forall A B C (f: A -> B -> C) al bl n,
+  length al = n -> length bl = n -> 
+  length (map2 f al bl) = n.
+Proof.
+induction al; destruct bl,n; simpl; intros; auto.
+inv H.
+Qed.
+
+Lemma length_rnd_64:
+  forall r k w, length r = 8 -> length (rnd_64 r k w) = 8.
+Proof.
+intros.
+revert r H w; induction k; simpl; intros; auto.
+unfold rnd_64; fold rnd_64.
+destruct w; auto.
+rename H into H0.
+repeat  (destruct r as [ | ? r]; rename H0 into H2; inv H2).
+apply IHk.
+reflexivity.
+Qed.
+
+Lemma length_process_block:
+  forall r b, length r = 8 -> length (process_block r b) = 8.
+Proof.
+ intros. unfold process_block.
+ unfold registers_add.
+ apply length_map2; auto.
+ apply length_rnd_64; auto.
+Qed.
+
+
+Lemma length_map2_add_rnd_64:
+ forall regs w,
+  length regs = 8 ->
+  length (map2 Int.add regs (rnd_64 regs K w)) = 8.
+Proof.
+ intros.
+ apply length_map2; auto.
+ apply length_rnd_64; auto.
+Qed.
+
+Lemma grab_and_process_block_length:
+ forall n r firstr msg r' m',
+    length r = 8 ->
+    length msg >= n ->
+    grab_and_process_block n r firstr msg  = (r',m') ->
+    length r' = 8.
+Proof.
+ induction n; intros.
+ inv H1.
+ apply length_process_block; auto.
+ destruct msg.
+ inv H0.
+ simpl in H0.
+ apply IHn in H1; auto.
+ omega.
+Qed.
+
+Lemma length_process_msg:
+  forall b, length (process_msg init_registers b) = 8.
+Proof.
+ intros.
+ assert (length init_registers = 8%nat) by reflexivity.
+ forget init_registers as regs.
+ assert (exists n, n >= length b)%nat by eauto.
+ destruct H0 as [n H0].
+ revert regs b H H0; induction n; intros; rewrite process_msg_equation.
+ destruct b; auto.
+ inv H0.
+ unfold grab_and_process_block.
+ repeat (destruct b; [apply H | ]).
+ apply IHn.
+ apply length_process_block; auto.
+ simpl in H0.
+ omega.
+Qed.
+
+Definition process_block_abs (b: list int) (a: s256abs) : s256abs :=
+match a with
+| S256abs hashed delta data =>
+    S256abs (hashed++b) (delta+ CBLOCK) data
+end.
+
+Definition init_s256abs : s256abs := S256abs nil 0 nil.
+
+Definition addlength_rel (n: nat) (a: s256abs) : s256abs :=
+ match a with S256abs hashed delta data =>
+     S256abs hashed (delta-n) data
+ end.
+
+Definition sha_finish (a a': s256abs) :=
+ match a, a' with
+ | S256abs hashed delta data,
+   S256abs hashed' delta' data' =>
+     hashed' = generate_and_pad (intlist_to_Zlist hashed ++ data) 0
+  /\ data'=nil /\ delta=0%nat /\ delta'=0
+ end.
+
+
+Fixpoint sequence (cs: list statement) s :=
+ match cs with
+ | nil => s
+ | c::cs' => Ssequence c (sequence cs' s)
+ end.
+
+Fixpoint rsequence (cs: list statement) s :=
+ match cs with
+ | nil => s
+ | c::cs' => Ssequence (rsequence cs' s) c
+ end.
+
+Lemma sequence_rsequence:
+ forall Espec Delta P cs s0 s R, 
+    @semax Espec Delta P (Ssequence s0 (sequence cs s)) R  <->
+  @semax Espec Delta P (Ssequence (rsequence (rev cs) s0) s) R.
+Proof.
+intros.
+revert Delta P R s0 s; induction cs; intros.
+simpl. apply iff_refl.
+simpl.
+rewrite seq_assoc.
+rewrite IHcs; clear IHcs.
+replace (rsequence (rev cs ++ [a]) s0) with
+    (rsequence (rev cs) (Ssequence s0 a)); [apply iff_refl | ].
+revert s0 a; induction (rev cs); simpl; intros; auto.
+rewrite IHl. auto.
+Qed.
+
+Lemma seq_assocN:  
+  forall {Espec: OracleKind},
+   forall Q Delta P cs s R,
+        @semax Espec Delta P (sequence cs Sskip) (normal_ret_assert Q) ->
+         @semax Espec 
+       (update_tycon Delta (sequence cs Sskip)) Q s R ->
+        @semax Espec Delta P (sequence cs s) R.
+Proof.
+intros.
+rewrite semax_skip_seq.
+rewrite sequence_rsequence.
+rewrite semax_skip_seq in H.
+rewrite sequence_rsequence in H.
+rewrite <- semax_seq_skip in H.
+eapply semax_seq'; [apply H | ].
+eapply semax_extensionality_Delta; try apply H0.
+clear.
+revert Delta; induction cs; simpl; intros.
+apply expr_lemmas.tycontext_sub_refl.
+eapply semax_lemmas.tycontext_sub_trans; [apply IHcs | ].
+clear.
+revert Delta; induction (rev cs); simpl; intros.
+apply expr_lemmas.tycontext_sub_refl.
+apply expr_lemmas.update_tycon_sub.
+apply IHl.
+Qed.
+
+Fixpoint sequenceN (n: nat) (s: statement) : list statement :=
+ match n, s with 
+ | S n', Ssequence a s' => a::sequenceN n' s'
+ | _, _ => nil
+ end.
+
+Lemma length_intlist_to_Zlist:
+  forall l, length (intlist_to_Zlist l) = (4 * length l).
+Proof.
+induction l.
+simpl. reflexivity. simpl. omega.
+Qed.
+
+Lemma process_msg_eq2:
+ forall regs hashed b,
+  length b = 16 ->
+ process_msg regs (b++hashed) =
+  process_msg (process_block regs (rev b)) hashed.
+Proof.
+intros.
+rewrite process_msg_equation.
+destruct (b++hashed) eqn:?.
+destruct b; inv H. inv Heql.
+rewrite <- Heql; clear i l Heql.
+unfold grab_and_process_block.
+rename H into H0.
+repeat (destruct b as [ | ?x b]; inv H0; rename H1 into H0).
+destruct b; inv H0.
+simpl. auto.
+Qed.
+
+Lemma process_msg_block:
+ forall (hashed b: list int), 
+   length b = LBLOCK ->
+   (exists n, length hashed = 16*n) ->
+   map2 Int.add (process_msg init_registers hashed)
+            (rnd_64 (process_msg init_registers hashed) K
+               (rev (generate_word (rev b) 48)))
+   = process_msg init_registers (hashed ++ b).
+Proof.
+intros.
+symmetry.
+destruct H0 as [n ?].
+change LBLOCK with 16 in H.
+transitivity (process_block (process_msg init_registers hashed) (rev b)) ; [ | reflexivity].
+forget init_registers as regs.
+revert hashed H0 b H regs; induction n; intros.
+*
+destruct hashed; inv H0.
+simpl app. 
+set (j :=  (rev (generate_word (rev b) 48))).
+rename H into H0.
+repeat (rename H0 into H2; destruct b as [ | ?x b]; inv H2).
+do 2 rewrite process_msg_equation.
+unfold grab_and_process_block.
+rewrite process_msg_equation.
+unfold j,process_block, registers_add. simpl rev.
+reflexivity.
+*
+rewrite mult_succ_r in H0. rewrite plus_comm in H0.
+rename H0 into H1.
+assert (exists hh, exists hashed', length hh = 16 /\ hashed=hh++hashed').
+do 16 (destruct hashed as [ | ?h hashed]; inv H1; rename H2 into H1).
+exists ([h,h0,h1,h2,h3,h4,h5,h6,h7,h8,h9,h10,h11,h12,h13,h14]), hashed.
+split; auto.
+destruct H0 as [hh [hashed' [? ?]]].
+subst.
+rewrite app_length in H1.
+assert (length hashed' = 16*n) by omega.
+clear H1.
+rewrite app_ass.
+rewrite process_msg_eq2 by auto.
+symmetry.
+rewrite process_msg_eq2 by auto.
+symmetry.
+apply IHn; auto.
+Qed.
+ 
+
+                  
+
+
+
