Makefile
@@ -105,7 +105,7 @@ FLOYD_FILES= \
 PROGS_FILES= \
   list_dt.v verif_reverse.v verif_queue.v verif_sumarray.v verif_message.v \
   insertionsort.v reverse.v queue.v sumarray.v message.v \
-  SHA256.v sha.v verif_sha.v entail_examples.v \
+  SHA256.v sha_lemmas.v sha.v verif_sha.v entail_examples.v \
   revarray.v verif_revarray.v 
 
 C_FILES = reverse.c queue.c sumarray.c message.c sha.c
